theories/SLFMore.v
@@ -789,3 +789,344 @@ Qed.
 
 
 
+
+(*
+
+(** * Heap entailment *)
+
+Set Implicit Arguments.
+Require Import LibCore TLCbuffer Fmap.
+Require Import Semantics SepBase.
+
+
+(** * Heap entailment *)
+
+CHANGE
+
+Notation "P ==> Q" := (pred_incl P Q)
+  (at level 55, right associativity) : heap_scope.
+
+(* [rel_incl'] is like TLC's [rel_incl] but defined in terms of [pred_incl]
+   so that after [intros r] we get an entailment. *)
+
+Definition rel_incl' A B (P Q:A->B->Prop) :=
+  forall r, pred_incl (P r) (Q r).
+
+Notation "P ===> Q" := (rel_incl' P Q)
+  (at level 55, right associativity) : heap_scope.
+
+Open Scope heap_scope.
+
+
+(* ---------------------------------------------------------------------- *)
+(* ** Examples of entailment *)
+
+
+r -> 6 * s -> 3 ==> s -> 3 * r -> 6
+
+FALSE : r -> 3 ==> s -> 4 * r -> 3
+
+negation: H1 h /\ ~ H2 h
+  ~ (s -> 4 * r -> 3)
+  forall h1 h2, ~ .. \/ ~ .. \/ ~ ...
+
+  ~ A \/ ~ B \/ ~ C
+  equiv to A -> B -> C -> False.
+
+  r -> 3 means h1 has domain r
+  s -> 4 means h2 has domain s
+
+  if r = s, then disjoint entails false
+  if r <> s, then h = h1 \u h2 = {r} \u {s}
+    dom h = {r}
+
+
+
+\[False] ==> r -> 6
+
+FALSE:   r -> 3 \* s -> 4 ==> \[False]
+
+r -> 3 \* r -> 4 ==> \[False]
+r -> 3 \* r -> 3 ==> \[False]
+
+
+
+
+
+
+(* ---------------------------------------------------------------------- *)
+(* ** Properties of entailment *)
+
+
+Section HimplProp.
+Variable A : Type.
+Implicit Types H : A -> Prop.
+
+Hint Unfold pred_incl.
+
+(** Entailment is reflexive, symmetric, transitive *)
+
+Lemma himpl_refl : forall H,
+  H ==> H.
+Proof using. intros h. auto. Qed.
+
+Lemma himpl_trans : forall H2 H1 H3,
+  (H1 ==> H2) ->
+  (H2 ==> H3) ->
+  (H1 ==> H3).
+Proof using. introv M1 M2. intros h H1h. eauto. Qed.
+
+Lemma himpl_antisym : forall H1 H2,
+  (H1 ==> H2) ->
+  (H2 ==> H1) ->
+  (H1 = H2).
+Proof using. introv M1 M2. applys pred_ext_1. intros h. iff*. Qed.
+
+(** Paragraphe of the definition, used by tactics *)
+
+Lemma himpl_inv : forall H1 H2 (h:A),
+  (H1 ==> H2) ->
+  (H1 h) ->
+  (H2 h).
+Proof using. auto. Qed.
+
+
+Lemma refl_rel_incl' : forall A B (Q:A->B->Prop),
+  Q ===> Q.
+Proof using. apply refl_rel_incl. Qed.
+
+
+
+(* ---------------------------------------------------------------------- *)
+(* ** A detour : extensionality *)
+
+(* SLIDE: extensionality *)
+
+
+
+
+
+
+(* ---------------------------------------------------------------------- *)
+(* ** Fundamental properties of hprop *)
+
+Lemma hstar_comm : forall H1 H2,
+   H1 \* H2 = H2 \* H1.
+Proof using.
+  intros H1 H2. unfold hprop, hstar. extens. intros h.
+  iff (h1&h2&M1&M2&D&U); rewrite~ heap_union_comm in U; exists* h2 h1.
+Qed.
+
+Lemma hstar_assoc : forall H1 H2 H3,
+  (H1 \* H2) \* H3 = H1 \* (H2 \* H3).
+Proof using.
+  intros H1 H2 H3. applys hprop_extens. intros h. split.
+  { intros (h'&h3&(h1&h2&M3&M4&D'&U')&M2&D&U). subst h'.
+    exists h1 (h2 \+ h3). splits~. { exists* h2 h3. } }
+  { intros (h1&h'&M1&(h2&h3&M3&M4&D'&U')&D&U). subst h'.
+    exists (h1 \+ h2) h3. splits~. { exists* h1 h2. } }
+Qed.
+
+Lemma hstar_hempty_l : forall H,
+  hempty \* H = H.
+Proof using.
+  intros. applys hprop_extens. intros h.
+  iff (h1&h2&M1&M2&D&U) M.
+  { forwards E: hempty_inv M1. subst.
+    rewrite~ heap_union_empty_l. }
+  { exists~ heap_empty h. }
+Qed.
+
+
+Lemma hstar_hexists : forall A (J:A->hprop) H,
+  (hexists J) \* H = hexists (fun x => (J x) \* H).
+Proof using.
+  intros. applys hprop_extens. intros h. iff M.
+  { destruct M as (h1&h2&(x&M1)&M2&D&U). exists~ x h1 h2. }
+  { destruct M as (x&(h1&h2&M1&M2&D&U)). exists h1 h2. splits~. exists~ x. }
+Qed.
+
+Lemma himpl_frame_l : forall H2 H1 H1',
+  H1 ==> H1' ->
+  (H1 \* H2) ==> (H1' \* H2).
+Proof using. introv W (h1&h2&?). exists* h1 h2. Qed.
+
+
+
+lemma transitive + frame
+  h1 ==> h2
+  x ==> h1 * r
+  h2 \* x => y
+  x==> y
+
+(* SLIDE: heap-entailment-properties *)
+
+
+(* ---------------------------------------------------------------------- *)
+(* ** example with instantiation and extrusion *)
+
+
+check out the "derived" states from previous chapter,
+and insert them here as exercises
+
+unfolding/folding of lists/trees give exercises
+
+split rule on segments
+
+
+r -> 6 ==> hexists n, r -> n \* even n
+
+hexists n, r -> n  ==> r --> 3   [FALSE]
+
+
+
+
+illustration for tactics:
+
+exists n , r -> n \* n > 0  ==>  exists n, n > 1 \* r -> (n-1)
+
+r -> 3 * s -> r ==> hexists n, r -> n * s -> n
+
+
+
+
+
+illustration for hchange
+
+lemma : r -> a \* r -> b = false.
+
+exists n, n > 0 \* n < 0 \* r -> n ==> r -> n * r -> n
+
+
+
+
+
+(* SLIDE: structural-rules *)
+
+
+(*--cover all structural rules*)
+(*--cover splitting rules for segments *)
+
+(* SLIDE: splitting-rule-for-list-segments *)
+
+
+
+
+
+(** * Separation algebra *)
+
+(** ** Entailment between heap predicates *)
+
+
+(** ** Equality between heap predicates *)
+
+
+
+(** ** [rew_heap] tactic *)
+
+(** ** Algebra of heap predicates *)
+
+(** ** Frame for heap predicates *)
+
+(* + simplification rule *)
+
+
+(** ** Extraction rules *)
+
+(** ** Examples of heap entailment *)
+
+(* + quiz *)
+
+
+(** ** Simplification tactic [himpl] *)
+
+(** ** Rewriting tactic [hchange] *)
+
+
+
+
+(* ---------------------------------------------------------------------- *)
+(* ** Frame and consequence *)
+
+Lemma triple_conseq : forall t H' Q' H Q,
+  H ==> H' ->
+  triple t H' Q' ->
+  Q' ===> Q ->
+  triple t H Q.
+Proof using.
+  introv MH M MQ. intros HF h N.
+  forwards (h'&v&R&K): (rm M) HF h. { hhsimpl~. }
+  exists h' v. splits~. { hhsimpl. hchanges (MQ v). }
+Qed.
+
+Lemma triple_frame : forall t H Q H',
+  triple t H Q ->
+  triple t (H \* H') (Q \*+ H').
+Proof using.
+  introv M. intros HF h N. rewrite hstar_assoc in N.
+  forwards (h'&v&R&K): (rm M) (H' \* HF) h. { hhsimpl~. }
+  exists h' v. splits~. { hhsimpl~. }
+Qed.
+
+
+check out the "derived" triples from previous chapter,
+and insert them here as exercises
+
+
+
+
+(* ---------------------------------------------------------------------- *)
+(* ** Extraction rules *)
+
+Lemma triple_hexists : forall t (A:Type) (J:A->hprop) Q,
+  (forall x, triple t (J x) Q) ->
+  triple t (hexists J) Q.
+Proof using.
+  introv M. intros HF h N. rewrite hstar_hexists in N.
+  destruct N as (x&N). applys* M.
+Qed.
+
+Lemma triple_hprop : forall t (P:Prop) H Q,
+  (P -> triple t H Q) ->
+  triple t (\[P] \* H) Q.
+Proof using.
+  intros t. applys (triple_hprop_from_hexists (triple t)).
+  applys triple_hexists.
+Qed.
+
+independent proofs
+
+as exercise, proof via the equivalence.
+
+
+(* ---------------------------------------------------------------------- *)
+(* ** Combined structural rule *)
+
+exercise
+
+(* ---------------------------------------------------------------------- *)
+(* ** Garbage collection *)
+
+support in hsimpl for \Top
+
+Lemma triple_htop_post : forall t H Q,
+  triple t H (Q \*+ \Top) ->
+  triple t H Q.
+Proof using.
+  introv M. intros HF h N. forwards* (h'&v&R&K): (rm M) HF h.
+  exists h' v. splits~. { rewrite <- htop_hstar_htop. hhsimpl. }
+Qed.
+
+Lemma triple_htop_pre : forall t H Q,
+  triple t H Q ->
+  triple t (H \* \Top) Q.
+Proof using.
+  introv M. applys triple_htop_post. applys~ triple_frame.
+Qed.
+
+
+
+
+
+
+*)
